\documentclass{article}
\usepackage[utf8]{inputenc}

\begin{document}

\section{$\beta-reduction$}
$((\lambda a.(\lambda b.b b) (\lambda b.b b)) b) ((\lambda c.(c b)) (\lambda a.a)) 
\to\\
((\lambda b.b b) (\lambda b.b b)) (((\lambda c.(c b)) (\lambda a.a))
\to\\
((\lambda b.b b) (\lambda b.b b)) ((\lambda a.a) b)
\to\\
(\lambda b.b b) (\lambda b.b b) b $

\section{S K K = I}
$(\lambda x.\lambda y.\lambda z.x z (y z)) (\lambda x.\lambda y.x) (\lambda x.\lambda y.x)
\to\\
(\lambda y.\lambda z.(\lambda x.\lambda y.x) z (y z)) (\lambda x.\lambda y.x)
\to\\ 
(\lambda y.\lambda z.(\lambda y.z) (y z)) (\lambda x.\lambda y.x)
\to\\ 
(\lambda y.\lambda z.z) (\lambda x.\lambda y.x)
\to\\
(\lambda z.z)$

\end{document}
